examples/pseudo_bool/cp_encoding/cp_to_ilp_allScript.sml
@@ -16,6 +16,7 @@ Ancestors
   cp_to_ilp_channeling
   cp_to_ilp_misc
   cp_to_ilp_scheduling
+  cp_to_ilp_sorting
 
 Definition encode_constraint_def:
   encode_constraint bnd c name =
@@ -30,6 +31,7 @@ Definition encode_constraint_def:
   | Channeling c => encode_channeling_constr bnd c name
   | Misc c => encode_misc_constr bnd c name
   | Scheduling c => encode_scheduling_constr bnd c name
+  | Sorting c => encode_sorting_constr bnd c name
 End
 
 Theorem encode_cp_one_sem_1:
@@ -51,6 +53,7 @@ Proof
   >- metis_tac[encode_channeling_constr_sem_1]
   >- metis_tac[encode_misc_constr_sem_1]
   >- metis_tac[encode_scheduling_constr_sem_1]
+  >- metis_tac[encode_sorting_constr_sem_1]
 QED
 
 Theorem encode_cp_one_sem_2:
@@ -70,6 +73,7 @@ Proof
   >- metis_tac[encode_channeling_constr_sem_2]
   >- metis_tac[encode_misc_constr_sem_2]
   >- metis_tac[encode_scheduling_constr_sem_2]
+  >- metis_tac[encode_sorting_constr_sem_2]
 QED
 
 (* An actual implementation will avoid duplicates here *)
@@ -119,6 +123,7 @@ Definition cencode_constraint_def:
   | Channeling c => cencode_channeling_constr bnd c name ec
   | Misc c => cencode_misc_constr bnd c name ec
   | Scheduling c => cencode_scheduling_constr bnd c name ec
+  | Sorting c => cencode_sorting_constr bnd c name ec
 End
 
 Theorem cencode_constraint_sem:
@@ -138,6 +143,7 @@ Proof
   >- metis_tac[cencode_channeling_constr_sem]
   >- metis_tac[cencode_misc_constr_sem]
   >- metis_tac[cencode_scheduling_constr_sem]
+  >- metis_tac[cencode_sorting_constr_sem]
 QED
 
 Definition cencode_constraints_def:
